verified boundary checking for power

CheckedArith.v
@@ -485,3 +485,423 @@ replace (- x mod 2 ^ 256 =? - x) with false. { trivial. }
 symmetry. rewrite Z.eqb_neq.
 intro H. apply Z.mod_small_iff in H; lia.
 Qed.
+
+
+(**********************************************************************
+ Binary search
+ **********************************************************************)
+
+
+
+(* This function descends slightly slower than a normal non-Coq implementation would,
+   meaning if we have 5 items to check, normally they would be split 2/3,
+   but we have to do 3/3 to make the recursion happy.
+ *)
+Fixpoint binary_search_rec (p: Z -> bool)
+                           (low: Z)
+                           (n: positive)
+{struct n}
+: Z
+:= match n with
+   | xH =>
+      let mid := low + 1 in
+      if p mid
+        then low
+        else mid
+   | xO half | xI half =>
+      let mid := low + Z.pos half + 1 in
+      if p mid
+        then binary_search_rec p low half
+        else binary_search_rec p mid half
+   end.
+
+Lemma binary_search_rec_lower (p: Z -> bool)
+                              (low: Z)
+                              (n: positive):
+  low <= binary_search_rec p low n.
+Proof.
+revert low. induction n; intro; cbn;
+  destruct p; try apply IHn;
+  try refine (Z.le_trans _ _ _ _ (IHn _)); lia.
+Qed.
+
+Lemma binary_search_rec_ok (p: Z -> bool)
+                           (low: Z)
+                           (n: positive)
+                           (Mono: forall x y, x < y -> p x = true -> p y = true)
+                           (LowOk: p low = false)
+                           (HighOk: p (low + Z.pos n + 1) = true):
+  let m := binary_search_rec p low n in
+  p m = false /\ p (Z.succ m) = true.
+Proof.
+revert low LowOk HighOk. induction n; intros.
+{ (* 2n + 1 *)
+  cbn.
+  remember (p (low + Z.pos n + 1)) as p_mid; symmetry in Heqp_mid; destruct p_mid.
+  { (* lower half *) now apply IHn. }
+  (* upper half *)
+  apply IHn. { assumption. }
+  replace (low + Z.pos n + 1 + Z.pos n + 1) with (low + Z.pos n~1 + 1) by lia.
+  assumption.
+}
+{ (* 2n *)
+  cbn.
+  remember (p (low + Z.pos n + 1)) as p_mid; symmetry in Heqp_mid; destruct p_mid.
+  { (* lower half *) now apply IHn. }
+  (* upper half *)
+  apply IHn. { assumption. }
+  refine (Mono _ _ _ HighOk).
+  lia.
+}
+(* 1 *)
+unfold m. cbn.
+remember (p (low + 1)) as p_mid; symmetry in Heqp_mid; now destruct p_mid.
+Qed.
+
+Lemma binary_search_rec_change (p q: Z -> bool)
+                               (low: Z)
+                               (n: positive)
+                               (ok: forall x, low < x -> p x = q x):
+  binary_search_rec p low n = binary_search_rec q low n.
+Proof.
+revert low ok. induction n; intros; cbn;
+  rewrite ok by lia; repeat rewrite IHn; trivial; intros; apply ok; lia.
+Qed.
+
+(** Perform binary search on a monotone boolean function [p]
+    which is false on [low] but true on [high].
+    Finds a number on which [p] is false but on the next one it's true.
+ *)
+Definition binary_search (p: Z -> bool)
+                         (low high: Z)
+: Z
+:= match high - low - 1 with
+   | Z0 => low
+   | Zpos n => binary_search_rec p low n
+   | Zneg _ => low (* bad arguments *)
+   end.
+
+Lemma binary_search_lower (p: Z -> bool)
+                          (low high: Z):
+  low <= binary_search p low high.
+Proof.
+unfold binary_search.
+destruct (high - low - 1); try apply Z.le_refl.
+apply binary_search_rec_lower.
+Qed.
+
+Lemma binary_search_ok (p: Z -> bool)
+                       (low high: Z)
+                       (Mono: forall x y, x < y -> p x = true -> p y = true)
+                       (LowOk: p low = false)
+                       (HighOk: p high = true):
+  let m := binary_search p low high in
+  p m = false /\ p (Z.succ m) = true.
+Proof.
+unfold binary_search.
+remember (high - low - 1) as d. symmetry in Heqd. destruct d as [|n|n].
+{ (* 0 *) assert (high = Z.succ low) by lia; now subst high. }
+{ (* pos *)
+  apply binary_search_rec_ok; try assumption.
+  assert (high = low + Z.pos n + 1) by lia.
+  now subst high.
+}
+(* neg *)
+(* this case contradicts [Mono] *)
+assert (LE: high <= low) by lia.
+apply Zle_lt_or_eq in LE.
+case LE; clear LE; intro LE.
+{ now rewrite (Mono _ _ LE HighOk) in LowOk. }
+subst. now rewrite LowOk in HighOk.
+Qed.
+
+Lemma binary_search_change (p q: Z -> bool)
+                           (low high: Z)
+                           (ok: forall x, low < x -> p x = q x):
+  binary_search p low high = binary_search q low high.
+Proof.
+unfold binary_search. destruct (high - low - 1); try easy.
+now rewrite (binary_search_rec_change p q) by apply ok.
+Qed.
+
+(******************************************************************************
+ * Powers and exponents
+ ******************************************************************************)
+
+(** Assuming [base > 2], compute the maximum allowed power before an overflow *)
+Definition uint256_max_power {C: VyperConfig} (base: Z)
+:= binary_search (fun x => 2 ^ 256 <=? Z.pow base x) 0 162.
+
+Lemma uint256_max_power_ok {C: VyperConfig} (base: Z) (BaseOk: 2 < base):
+  let p := uint256_max_power base in
+  Z.pow base p < 2 ^ 256 /\ 2 ^ 256 <= Z.pow base (Z.succ p).
+Proof.
+unfold uint256_max_power.
+remember (fun x : Z => 2 ^ 256 <=? base ^ x) as f.
+assert (F0: f 0 = false) by now subst f.
+assert (F162: f 162 = true).
+{
+  subst f.
+  apply Z.leb_le.
+  assert (T: 2 ^ 256 <= 3 ^ 162) by now apply Z.leb_le.
+  apply (Z.le_trans _ _ _ T).
+  apply Z.pow_le_mono_l.
+  lia.
+}
+assert (Mono: forall x y, x < y -> f x = true -> f y = true).
+{
+  intros. subst f.
+  rewrite Z.leb_le in *.
+  apply (Z.le_trans (2 ^ 256) (base ^ x) (base ^ y)). { assumption. }
+  apply Z.pow_le_mono_r; lia.
+}
+assert (B := binary_search_ok f 0 162 Mono F0 F162).
+subst f. cbn zeta in B.
+rewrite Z.leb_gt in B. rewrite Z.leb_le in B.
+apply B.
+Qed.
+
+(** Unchecked power modulo [2^256]. *)
+Definition uint256_pow {C: VyperConfig} (a b: uint256)
+: uint256
+:= uint256_of_Z (Z_of_uint256 a ^ Z_of_uint256 b).
+
+(** This is checked power with a constant base close to how it's compiled:
+    for [base == 0]: [pow == 0]
+    for [base == 1]: [pow; 1]
+    for [base == 2]: [assert pow < 256; 1 << pow]
+    for [base >= 3]: [assert pow <= uint256_max_power base; base ** pow
+ *)
+Definition uint256_checked_pow_const_base {C: VyperConfig} (base pow: uint256)
+: option uint256
+:= let base_Z := Z_of_uint256 base in
+   let pow_Z := Z_of_uint256 pow in
+   if base_Z =? 0 then Some (if pow_Z =? 0 then one256 else zero256) else
+   if base_Z =? 1 then Some one256 else
+   if base_Z =? 2
+     then if pow_Z <? 256
+            then Some (uint256_shl one256 pow)
+            else None
+     else if pow_Z <=? uint256_max_power base_Z
+            then Some (uint256_pow base pow)
+            else None.
+
+Lemma uint256_checked_pow_const_base_ok {C: VyperConfig} (base pow: uint256):
+  uint256_checked_pow_const_base base pow = interpret_binop Pow base pow.
+Proof.
+cbn. unfold uint256_checked_pow_const_base. unfold maybe_uint256_of_Z.
+rewrite uint256_ok.
+remember (Z_of_uint256 base =? 0) as base_0. symmetry in Heqbase_0. destruct base_0.
+{ (* 0 ^ pow *)
+  rewrite Z.eqb_eq in Heqbase_0.
+  rewrite Heqbase_0.
+  remember (Z_of_uint256 pow =? 0) as pow_0. symmetry in Heqpow_0. destruct pow_0.
+  { (* 0 ^ 0 == 1 *)
+    rewrite Z.eqb_eq in Heqpow_0.
+    now rewrite Heqpow_0.
+  }
+  rewrite Z.eqb_neq in Heqpow_0.
+  apply Z.pow_0_l' in Heqpow_0. 
+  now rewrite Heqpow_0.
+}
+rewrite Z.eqb_neq in Heqbase_0.
+remember (Z_of_uint256 base =? 1) as base_1. symmetry in Heqbase_1. destruct base_1.
+{ (* 1 ^ pow *)
+  rewrite Z.eqb_eq in Heqbase_1.
+  rewrite Heqbase_1.
+  rewrite Z.pow_1_l. { easy. }
+  apply uint256_range.
+}
+rewrite Z.eqb_neq in Heqbase_1.
+remember (Z_of_uint256 base =? 2) as base_2. symmetry in Heqbase_2. destruct base_2.
+{ (* 2 ^ pow *)
+  rewrite Z.eqb_eq in Heqbase_2.
+  rewrite Heqbase_2.
+  unfold uint256_shl.
+  replace (Z_of_uint256 one256) with 1 by (unfold one256; now rewrite uint256_ok).
+  rewrite Z.shiftl_1_l.
+  remember (2 ^ Z_of_uint256 pow mod 2 ^ 256 =? 2 ^ Z_of_uint256 pow) as m. symmetry in Heqm.
+  assert (T: 2 ^ 256 <> 0) by discriminate.
+  assert (M := Z.mod_small_iff (2 ^ Z_of_uint256 pow) (2 ^ 256) T). clear T.
+  assert (R := uint256_range pow).
+  assert (NN: ~(2 ^ 256 < 2 ^ Z_of_uint256 pow <= 0)) by lia.
+  assert (L: 0 <= 2 ^ Z_of_uint256 pow) by now apply Z.pow_nonneg.
+  assert (MM: 2 ^ Z_of_uint256 pow mod 2 ^ 256 = 2 ^ Z_of_uint256 pow 
+               <->
+              2 ^ Z_of_uint256 pow < 2 ^ 256) by tauto.
+  clear M NN.
+  assert (Q: 2 ^ Z_of_uint256 pow < 2 ^ 256 <-> Z_of_uint256 pow < 256).
+  { symmetry. now apply Z.pow_lt_mono_r_iff. }
+  assert (P: 2 ^ Z_of_uint256 pow mod 2 ^ 256 = 2 ^ Z_of_uint256 pow 
+              <->
+             Z_of_uint256 pow < 256) by tauto.
+  clear MM Q.
+  remember (Z_of_uint256 pow <? 256) as l. symmetry in Heql.
+  destruct l, m; try rewrite Z.ltb_lt in *; try rewrite Z.ltb_ge in *;
+                 try rewrite Z.eqb_eq in *; try rewrite Z.eqb_neq in *; trivial.
+  { tauto. }
+  apply P in Heqm. lia.
+}
+rewrite Z.eqb_neq in Heqbase_2.
+(* base ^ pow, base >= 3 *)
+assert (L: 2 < Z_of_uint256 base). { assert (R := uint256_range base). lia. }
+assert (M := uint256_max_power_ok _ L).
+unfold uint256_pow.
+remember (Z_of_uint256 base ^ Z_of_uint256 pow mod 2 ^ 256 
+           =?
+          Z_of_uint256 base ^ Z_of_uint256 pow) as m.
+symmetry in Heqm.
+remember (Z_of_uint256 pow <=? uint256_max_power (Z_of_uint256 base)) as l. symmetry in Heql.
+enough (H: m = l) by now rewrite H.
+destruct l.
+{
+  rewrite Z.leb_le in Heql.
+  subst m.
+  rewrite Z.eqb_eq.
+  apply Z.mod_small.
+  split. { apply Z.pow_nonneg. lia. }
+  refine (Z.le_lt_trans _ _ _ _ (proj1 M)).
+  apply Z.pow_le_mono_r. { lia. } exact Heql.
+}
+rewrite Z.leb_gt in Heql.
+subst m. rewrite Z.eqb_neq. intro H.
+apply Z.mod_small_iff in H. 2:discriminate.
+enough (2 ^ 256 <= Z_of_uint256 base ^ Z_of_uint256 pow) by lia.
+clear H.
+apply (Z.le_trans _ _ _ (proj2 M)).
+apply Z.pow_le_mono_r; lia.
+Qed.
+
+
+(** Assuming [pow >= 2], compute the maximum allowed base before an overflow *)
+Definition uint256_max_base {C: VyperConfig} (pow: Z)
+:= binary_search (fun x => 2 ^ 256 <=? Z.pow x pow) 0 (2 ^ 128).
+
+Lemma uint256_max_base_ok {C: VyperConfig} (pow: Z) (PowOk: 2 <= pow):
+  let b := uint256_max_base pow in
+  Z.pow b pow < 2 ^ 256 /\ 2 ^ 256 <= Z.pow (Z.succ b) pow.
+Proof.
+unfold uint256_max_base.
+remember (fun x : Z => 2 ^ 256 <=? x ^ pow) as f.
+pose (g := fun x => ((0 <=? x) && f x)%bool).
+assert (E: binary_search f 0 (2 ^ 128) = binary_search g 0 (2 ^ 128)).
+{
+  apply binary_search_change.
+  intros x L.
+  subst f g.
+  cbn beta.
+  apply Z.lt_le_incl in L.
+  apply Z.leb_le in L.
+  rewrite L.
+  apply Bool.andb_true_l.
+}
+rewrite E.
+assert (Low: g 0 = false).
+{
+  subst g. subst f.
+  replace (0 ^ pow) with 0. 2:{ symmetry. apply Z.pow_0_l. lia. }
+  easy.
+}
+assert (High: g (2 ^ 128) = true).
+{
+  subst g. subst f.
+  apply Z.leb_le.
+  replace (2 ^ 256) with ((2 ^ 128) ^ 2) by trivial.
+  now apply Z.pow_le_mono_r.
+}
+assert (Mono: forall x y, x < y -> g x = true -> g y = true).
+{
+  intros x y XY H. subst g. subst f.
+  rewrite Bool.andb_true_iff in *.
+  destruct H as (PosX, H).
+  split; rewrite Z.leb_le in *; try lia.
+  apply (Z.le_trans (2 ^ 256) (x ^ pow) (y ^ pow)). { assumption. }
+  apply Z.pow_le_mono_l; lia.
+}
+assert (B := binary_search_ok g _ _ Mono Low High).
+cbn zeta in B. destruct B as (U, V).
+rewrite<- E in *.
+assert (L := binary_search_lower f 0 (2 ^ 128)).
+remember (binary_search f 0 (2 ^ 128)) as x.
+subst g. cbn in U. cbn in V.
+assert (L': 0 <= Z.succ x) by lia.
+rewrite<- Z.leb_le in L.
+rewrite<- Z.leb_le in L'.
+rewrite L in U. rewrite L' in V.
+cbn in U. cbn in V.
+subst f.
+apply Z.leb_gt in U. apply Z.leb_le in V.
+tauto.
+Qed.
+
+(** This is ugly but there's no extensionality requirement for uint256s,
+    so [base ** 1] is not exactly the same as [base]. *)
+Definition uint256_unary_plus {C: VyperConfig} (a: uint256)
+:= uint256_of_Z (Z_of_uint256 a).
+
+(** This is checked power with a constant exponent close to how it's compiled:
+    for [pow == 0]: [base; 1]
+    for [pow == 1]: [+base]
+    for [pow >= 2]: [assert base <= uint256_max_base pow; base ** pow
+ *)
+Definition uint256_checked_pow_const_exponent {C: VyperConfig} (base pow: uint256)
+: option uint256
+:= let base_Z := Z_of_uint256 base in
+   let pow_Z := Z_of_uint256 pow in
+   if pow_Z =? 0 then Some one256 else
+   if pow_Z =? 1 then Some (uint256_unary_plus base) else
+   if base_Z <=? uint256_max_base pow_Z
+     then Some (uint256_pow base pow)
+     else None.
+
+Lemma uint256_checked_pow_const_exponent_ok {C: VyperConfig} (base pow: uint256):
+  uint256_checked_pow_const_exponent base pow = interpret_binop Pow base pow.
+Proof.
+cbn. unfold uint256_checked_pow_const_exponent. unfold maybe_uint256_of_Z.
+rewrite uint256_ok.
+remember (Z_of_uint256 pow =? 0) as pow_0. symmetry in Heqpow_0. destruct pow_0.
+{ (* base ^ 0 *)
+  rewrite Z.eqb_eq in Heqpow_0. rewrite Heqpow_0.
+  now rewrite Z.pow_0_r.
+}
+rewrite Z.eqb_neq in Heqpow_0.
+remember (Z_of_uint256 pow =? 1) as pow_1. symmetry in Heqpow_1. destruct pow_1.
+{ (* base ^ 1 *)
+  rewrite Z.eqb_eq in Heqpow_1. rewrite Heqpow_1.
+  rewrite Z.pow_1_r.
+  assert (R := Z.mod_small _ _ (uint256_range base)).
+  rewrite<- Z.eqb_eq in R.
+  now rewrite R.
+}
+rewrite Z.eqb_neq in Heqpow_1.
+assert (L: 2 <= Z_of_uint256 pow) by (assert (R := uint256_range pow); lia).
+assert (B := uint256_max_base_ok _ L).
+remember (Z_of_uint256 base ^ Z_of_uint256 pow mod 2 ^ 256 
+           =?
+          Z_of_uint256 base ^ Z_of_uint256 pow) as m.
+symmetry in Heqm.
+remember (Z_of_uint256 base <=? uint256_max_base (Z_of_uint256 pow)) as l. symmetry in Heql.
+enough (H: m = l) by now rewrite H.
+assert (R := uint256_range base).
+destruct l.
+{
+  rewrite Z.leb_le in Heql.
+  subst m.
+  rewrite Z.eqb_eq.
+  apply Z.mod_small.
+  split. { apply Z.pow_nonneg. tauto. }
+  refine (Z.le_lt_trans _ _ _ _ (proj1 B)).
+  apply Z.pow_le_mono_l. lia.
+}
+rewrite Z.leb_gt in Heql.
+subst m. rewrite Z.eqb_neq. intro H.
+apply Z.mod_small_iff in H. 2:discriminate.
+enough (2 ^ 256 <= Z_of_uint256 base ^ Z_of_uint256 pow) by lia.
+clear H.
+apply (Z.le_trans _ _ _ (proj2 B)).
+apply Z.pow_le_mono_l.
+split. 2:lia.
+enough (0 <= uint256_max_base (Z_of_uint256 pow)) by lia.
+unfold uint256_max_base.
+apply binary_search_lower.
+Qed.
